theories/elpi_equiv.v
@@ -7,10 +7,10 @@ Section NurEqiv.
   Variable (u : Unif).
   Variable (p : program).
 
-  Lemma tree_to_elpi fv A s1 B s2 b s0:
+  Lemma tree_to_elpi fv A s1 B s2 b s0 fv':
     vars_tree A `<=` fv -> vars_sigma s1 `<=` fv ->
     valid_tree A ->
-      run u p fv s1 A (Some s2) B b -> 
+      run u p fv s1 A (Some s2) B b fv' -> 
         exists x xs,
           t2l A s1 nilC = x ::: xs /\
           nur u p fv x.1 x.2 xs s2 (t2l (odflt Dead B) s0 nilC).
@@ -22,7 +22,7 @@ Section NurEqiv.
       rewrite (success_t2l sIgn)//.
       repeat eexists.
       apply: StopE.
-    + move=> s1 s2 r A B n fv fv' eA rB IH s4 ? sIgn fvP1 fvP2 vA; subst.
+    + move=> s1 s2 r A B n fv fv' ? eA rB IH s4 ? sIgn fvP1 fvP2 vA; subst.
       have ?:= tree_fv_step_cut eA; subst.
       have {IH} //= [|[sy y]/=[ys [+ H4]]]:= IH _ erefl sIgn _ fvP2 (valid_tree_step vA eA).
         by apply/fsubset_trans/fvP1/vars_tree_step_cut/eA.
@@ -30,7 +30,7 @@ Section NurEqiv.
       have [x[tl[H1 H2]]] := [elaborate s2l_CutBrothers s1 nilC vA eA].
       rewrite H1 H2 H5 => -[???]; subst.
       repeat eexists; by apply CutE.
-    + move=> s1 s2 r A B n fv fv' eA rB IH s4 ? sIgn fvP1 fvP2 vA; subst. 
+    + move=> s1 s2 r A B n fv fv' ? eA rB IH s4 ? sIgn fvP1 fvP2 vA; subst. 
       have /=vB:= (valid_tree_step vA eA). 
       have fA := step_not_failed eA notF.
       have [s[x[xs +]]] := failed_t2l vA fA s1 nilC.
@@ -54,7 +54,7 @@ Section NurEqiv.
       have [[[? SS] H1]] := s2l_Expanded_cut vA eA H; subst.
       rewrite cats0 => ->[???]; subst.
       by apply: CutE.
-    + move=> s1 s2 A B r n fv fA nA H IH s3 ? sIgn fvP1 fvP2 vA; subst.
+    + move=> s1 s2 A B r n fv ? fA nA H IH s3 ? sIgn fvP1 fvP2 vA; subst.
       have vB := valid_tree_next_alt vA nA.
       have H1 := failed_next_alt_some_t2l _ vA fA nA.
       have {}fvP := vars_tree_next_alt_sub_flow fvP1 nA.
@@ -66,7 +66,7 @@ Section NurEqiv.
 Lemma elpi_to_tree fv s1 s2 a na g  : 
   nur u p fv s1 g a s2 na -> 
   forall s0 t, valid_tree t -> (t2l t s0 nilC) = ((s1,g) ::: a) -> 
-  exists t1 n, run u p fv s0 t (Some s2) t1 n /\ t2l (odflt Dead t1) s0 nilC = na.
+  exists t1 n fv2, run u p fv s0 t (Some s2) t1 n fv2 /\ t2l (odflt Dead t1) s0 nilC = na.
 Proof.
   elim; clear.
   - move=> s a fv s1 A vA /= H.
@@ -100,7 +100,7 @@ Proof.
         case X: (step u p fv s A') => [[fv' r'] A''].
         have:= next_cut_s2l fA' vA' H X => /=.
         rewrite clean_ca_nil/= => -[H1 H2].
-        have /= [t1[n [{}IH H3]]] := IH _ _ (valid_tree_step vA' X) H1; subst.
+        have /= [t1[n [fv0[{}IH H3]]]] := IH _ _ (valid_tree_step vA' X) H1; subst.
         move: H2; case: ifP => Hx [??]; subst.
           repeat eexists.
           apply: run_fail fA nA _.
@@ -112,7 +112,7 @@ Proof.
       case X: (step u p fv s A) => [[fv' r'] A'].
       have:= next_cut_s2l fA vA H X => /=.
       rewrite clean_ca_nil/= => -[H1 H2].
-      have /= [t1[n [{}IH H3]]] := IH _ _ (valid_tree_step vA X) H1; subst.
+      have /= [t1[n[fv0[{}IH H3]]]] := IH _ _ (valid_tree_step vA X) H1; subst.
       move: H2; case: ifP => Hx [??]; subst.
         repeat eexists.
         by apply: run_cut IH.
@@ -131,14 +131,14 @@ Proof.
         have /= vA' := (valid_tree_next_alt vA nA).
         have [] := next_callS_s2l p u fv fA' vA' H.
         rewrite B/=clean_ca_nil => H1 H2.
-        have /= [t1[n [{}IH ?]]] := IH _ _ (valid_tree_step vA' erefl) H1; subst.
+        have /= [t1[n[fv0[{}IH ?]]]] := IH _ _ (valid_tree_step vA' erefl) H1; subst.
         repeat eexists.
         apply: run_fail fA nA _.
         apply: run_step H2 IH.
       rewrite -(@clean_ca_nil (t2l _ _ _)) in H.
       have [] := next_callS_s2l p u fv fA vA H.
       rewrite B/= clean_ca_nil/= => H1 H2.
-      have /= [t1[n [{}IH ?]]] := IH _ _ (valid_tree_step vA erefl) H1; subst.
+      have /= [t1[n [?[{}IH ?]]]] := IH _ _ (valid_tree_step vA erefl) H1; subst.
       repeat eexists.
       apply: run_step H2 IH.
     }
@@ -154,14 +154,14 @@ Proof.
         rewrite -(@clean_ca_nil (t2l _ _ _)) in H.
         have [] := next_callS_s2l p u fv fA' vA' H.
         rewrite B/= clean_ca_nil/= cat0s => H1 H2.
-        have /= [t1[n [{}IH ?]]] := IH _ _ (valid_tree_step vA' erefl) H1; subst.
+        have /= [t1[n[?[{}IH ?]]]] := IH _ _ (valid_tree_step vA' erefl) H1; subst.
         repeat eexists.
         apply: run_fail fA nA _.
         apply: run_step H2 IH.
       rewrite -(@clean_ca_nil (t2l _ _ _)) in H.
       have [] := next_callS_s2l p u fv fA vA H.
       rewrite B/= clean_ca_nil/=cat0s => H1 H2.
-      have /= [t1[n [{}IH ?]]] := IH _ _ (valid_tree_step vA erefl) H1; subst.
+      have /= [t1[n[?[{}IH ?]]]] := IH _ _ (valid_tree_step vA erefl) H1; subst.
       repeat eexists.
       apply: run_step H2 IH.
     }
